% Preamble
\documentclass[12pt]{simple_doc}

% Packages
\usepackage{amsmath}
\usepackage{amssymb}
\usepackage{simple_note}
\usepackage{enumitem}
\usepackage{tkz-euclide}

% Document
\begin{document}
    \exerheader{Statistics}{EV of Min Pairs}{\today}{ctbBlueDark}

    Authors: Mingxiao Hu, Bo Zhang

    \begin{cbstripe}{Problem}{ctbGreenDark}{ctbGreenLight}
        \textit{Given three random variables $X$, $Y$, $Z$ over uniform distribution $U(0, 1)$. Find
        the expectation of $W = \min(X + Y, Y + Z)$.}
    \end{cbstripe}

    \begin{equation*}
		\begin{aligned}
		\mathbb{E}(W) &= \mathbb{E}\Big[(X + Y)I(X < Z)\Big] + \mathbb{E}\Big[(Y + Z)I(Z < X)\Big] \\
		   &= \mathbb{E}\Big[X\cdot I(X < Z)\Big] + \mathbb{E}\Big[Y\cdot I(X < Z)\Big]
                + \mathbb{E}\Big[Y\cdot I(Z < X)\Big] + \mathbb{E}\Big[Z\cdot I(Z < X)\Big]\\
           &= \mathbb{E}[Y] + 2 \mathbb{E}\Big[X\cdot I(X < Z)\Big] \\
           &= \frac{1}{2} + 2 \int_0^1 \int_0^z xdxdz \\
           &= \frac{1}{2} + \int_0^1 z^2 dz \\
           &= \frac{1}{2} + \frac{1}{3} \\
           &= \frac{5}{6}
		\end{aligned}
	\end{equation*}


    \begin{cbstripe}{Problem}{ctbPinkDark}{ctbPinkLight}
        \textit{Given five random variables $a, b, c, d, e$ over uniform distribution $U(0, 1)$. Find
        the expectation of $Z = \min(a + b, b + c, c + d, d + e)$.}
    \end{cbstripe}

    Let $X = \min(a + b, b + c)$ and $Y = \min(c + d, d + e)$, Then
    \begin{equation*}
        \mathbb{E}[Z] = \mathbb{E}\Big[\mathbb{E}\big[\min(X, Y)|c\big]\Big]
            = \int_0^1 \mathbb{E}\big[\min(X, Y)|c\big]dc
    \end{equation*}

    Simplify the integrand,
    \begin{equation*}
        \begin{aligned}
        \mathbb{E}[min(X, Y)|c] &= \int_0^{1 + c} P(\min(X, Y) \geqslant x | c) dx\\
            &= \int_0^{1 + c} P(X \geqslant x | c) \cdot P(Y \geqslant x | c) dx\\
            &= \int_0^{1 + c} P^2 (X \geqslant x | c)  dx
        \end{aligned}
    \end{equation*}

    Inside the integral,
    \begin{equation*}
        \begin{aligned}
        P(X \geqslant x | c) &= P((a + b \geqslant x, b + c \geqslant x)|c)\\
            &= \int_{(x-c)^+}^1 \int_{(x-b)^+}^1 da db\\
            &= \int_{(x-c)^+}^1 (1 - (x-b)^+) db
        \end{aligned}
    \end{equation*}

    When $0 \leqslant x \leqslant c$, the above integral becomes
    \begin{equation*}
        \int_0^x (1 - (x-b)) db + \int_x^1 db = 1 - \frac{x^2}{2}
    \end{equation*}

    When $c \leqslant x \leqslant 1$, the above integral becomes
    \begin{equation*}
        \int_{x-c}^x (1 - (x-b)) db + \int_x^1 db = 1 - x + c - \frac{c^2}{2}
    \end{equation*}

    When $1 \leqslant x \leqslant 1 + c$, the above integral becomes
    \begin{equation*}
        \int_{x-c}^1 (1 - (x-b)) db = \frac{3}{2} - 2x + \frac{x^2}{2} + c - \frac{c^2}{2}
    \end{equation*}

    Now the expectation can be rewritten as
    \begin{equation*}
        \mathbb{E}[Z] = \int_0^1 G(c) dc
    \end{equation*}
    where the integrand is
    \begin{equation*}
        G(c) = \int_0^{1 + c} S^2(x, c) dx
    \end{equation*}
    and
    \begin{equation*}
        S(x, c) =
            \begin{cases}
              1 - \frac{x^2}{2}, & \text{when}\ 0 \leqslant x \leqslant c\\
              1 - x + c - \frac{c^2}{2}, & \text{when}\ c \leqslant x \leqslant 1\\
              \frac{3}{2} - 2x + \frac{x^2}{2} + c - \frac{c^2}{2}, & \text{when}\ 1 \leqslant x \leqslant 1 + c
            \end{cases}
    \end{equation*}

    \medskip
    \textbf{Solution 1: Integration by parts}\\
    Note that
    \begin{equation*}
        \begin{aligned}
            G(c) &= \int_0^{1 + c} S^2(x, c) dx = xS^2(x, c)\biggr\rvert_0^{1+c}
                    - \int_0^{1 + c} 2xS(x,c)S_x^{'}(x,c) dx\\
                 &= \int_0^{1 + c} -2xS(x,c)S_x^{'}(x,c) dx
        \end{aligned}
    \end{equation*}
    To derive the integrand, from Equation (10)
    \begin{equation*}
        S_x^{'}(x, c) =
            \begin{cases}
              -x, & \text{when}\ 0 \leqslant x \leqslant c\\
              -1, & \text{when}\ c \leqslant x \leqslant 1\\
              -2 +x, & \text{when}\ 1 \leqslant x \leqslant 1 + c
            \end{cases}
    \end{equation*}
    then the integrand is
    \begin{equation*}
        T(x, c) = -2xS(x, c)S_x^{'}(x, c) =
            \begin{cases}
              2x^2 - x^4, &\\
              2x - 2x^2 + x(2c - c^2), &\\
              -x^4 +6x^3 -8x^2 + (2x - x^2)(3 + 2c - c^2), &
            \end{cases}
    \end{equation*}

    Now we compute each case.

    When $0 \leqslant x \leqslant c$,
    \begin{equation*}
        T_1(x, c) = 2x^2 - x^4
    \end{equation*}
    then
    \begin{equation*}
		\begin{aligned}
		G_1(c) &= \int_0^c T_1(x, c) dx \\
		   &= \int_0^c (2x^2 - x^4) dx\\
           &= \frac{2c^3}{3} - \frac{c^5}{5}
		\end{aligned}
	\end{equation*}
    and
    \begin{equation*}
        E_1 = \int_0^1 G_1(c)dc = \frac{2}{12} - \frac{1}{30} = \frac{2}{15}
    \end{equation*}

    Similarly, when $c \leqslant x \leqslant 1$,
    \begin{equation*}
        T_2(x, c) = 2x - 2x^2 + x(2c - c^2)
    \end{equation*}
    then
    \begin{equation*}
		\begin{aligned}
		G_2(c) &= \int_c^1 T_2(x, c) dx \\
		   &= \int_c^1 [- 2x^2 + x(2 + 2c - c^2)] dx\\
           &= -\frac{2}{3} + \frac{2c^3}{3} + 2 + 2c -c^2 -c^2(2 + 2c - c^2)
           &= \frac{1}{3} + c - \frac{3c^2}{2} - \frac{c^3}{3} + \frac{c^4}{2}
		\end{aligned}
    \end{equation*}
    and
    \begin{equation*}
        E_2 = \int_0^1 G_2(c)dc = \frac{1}{3} + \frac{1}{2}  - \frac{1}{2}
            - \frac{1}{12} + \frac{1}{10} = \frac{7}{20}
    \end{equation*}

    When $1 \leqslant x \leqslant 1 + c$,
    \begin{equation*}
        T_3(x, c) = -x^4 +6x^3 -8x^2 + (2x - x^2)(3 + 2c - c^2)
    \end{equation*}
    then
    \begin{equation*}
		\begin{aligned}
		G_3(c) &= \int_1^{1+c} T_3(x, c) dx \\
		   &= \int_1^{1+c} [-x^4 +6x^3 -8x^2 + (2x - x^2)(3 + 2c - c^2)] dx\\
           &= -\frac{1}{5}[(1+c)^5 - 1] + \frac{3}{2}[(1+c)^4 - 1] - \frac{8}{3}[(1+c)^3 - 1]\\
           &\ \ \ + \{[(1+c)^2 - 1] - \frac{1}{3}[(1+c)^3 - 1]\}(3 + 2c - c62)\\
           &= \frac{41}{30} - \frac{1}{5}(1+c)^5 + \frac{3}{2}(1+c)^4 - \frac{8}{3}(1+c)^3\\
           &\ \ \ + (-\frac{c^3}{3} + c)(3 + 2c - c^2)\\
           &= \frac{41}{30} - \frac{1}{5}(1+c)^5 + \frac{3}{2}(1+c)^4 - \frac{8}{3}(1+c)^3\\
           &\ \ \ + \frac{c^5}{3} - \frac{2c^4}{3} -2c^3 + 2c^2 + 3c
		\end{aligned}
    \end{equation*}
    and
    \begin{equation*}
        \begin{aligned}
        E_3 &= \int_0^1 G_3(c)dc = \frac{41}{30} - \frac{1}{30}[2^6 - 1] + \frac{3}{10}[2^5 - 1]
                - \frac{2}{3}[2^4 - 1] + \frac{1}{18} - \frac{2}{15} - \frac{1}{2}
                + \frac{2}{3} + \frac{3}{2}\\
            &= \frac{1}{10} + \frac{1}{18}\\
            &= \frac{14}{90}
        \end{aligned}
    \end{equation*}

    Finally,
    \begin{equation*}
        \mathbb{E}[Z] = E_1 + E_2 + E_3 = \frac{2}{15} + \frac{7}{20} + \frac{14}{90}
                      = \frac{23}{36} = 0.63\overline{8}
    \end{equation*}


    \medskip
    \textbf{Solution 2: Without integration by parts}\\
    When $0 \leqslant x \leqslant c$,
    \begin{equation*}
        S_1(x, c) = 1 - \frac{x^2}{2}
    \end{equation*}
    then
    \begin{equation*}
		\begin{aligned}
		G_1(c) &= \int_0^c S_1^2(x, c) dx \\
		   &= \int_0^c (1 - x^2 + \frac{x^4}{4}) dx\\
           &= c - \frac{c^3}{3} + \frac{c^5}{20}
		\end{aligned}
	\end{equation*}
    and
    \begin{equation*}
		\begin{aligned}
		E_1 &= \int_0^1 G_1(c) dc \\
		   &= \int_0^1 ( c - \frac{c^3}{3} + \frac{c^5}{20}) dc\\
           &= \frac{1}{2} - \frac{1}{12} + \frac{1}{120}\\
           &= \frac{17}{40}
		\end{aligned}
	\end{equation*}

    When $c \leqslant x \leqslant 1$,
    \begin{equation*}
        S_2(x, c) = 1 + c - \frac{c^2}{2} - x
    \end{equation*}
    then
    \begin{equation*}
		\begin{aligned}
		G_2(c) &= \int_c^1 S_2^2(x, c) dx \\
		   &= \int_c^1 [(1 + c - \frac{c^2}{2})^2 - 2x(1 + c - \frac{c^2}{2}) + x^2] dx\\
           &= (1 + c - \frac{c^2}{2})^2 - (1 + c - \frac{c^2}{2}) + \frac{1}{3}
             - c(1 + c - \frac{c^2}{2})^2 + c^2(1 + c - \frac{c^2}{2}) - \frac{c^3}{3}\\
           &= \frac{1}{3} - \frac{c^2}{2} - \frac{c^3}{3} + \frac{3c^4}{4} - \frac{c^5}{4}\\
		\end{aligned}
	\end{equation*}
    and
    \begin{equation*}
		\begin{aligned}
		E_2 &= \int_0^1 G_2(c) dc \\
		   &= \frac{1}{3} - \frac{1}{6} - \frac{1}{12} + \frac{3}{20} - \frac{1}{24}\\
           &= \frac{23}{120}
		\end{aligned}
	\end{equation*}

    When $1 \leqslant x \leqslant 1 + c$,
    \begin{equation*}
        S_3(x, c) = \frac{x^2}{2} - 2x + \frac{3}{2} + c - \frac{c^2}{2}
    \end{equation*}
    then
    \begin{equation*}
		\begin{aligned}
		G_3(c) &= \int_1^{1+c} S_3^2(x, c) dx \\
		   &= \int_1^{1+c} [\frac{x^4}{4} - 2x^3 + 4x^2 + x^2(\frac{3}{2} + c - \frac{c^2}{2})
              -4x(\frac{3}{2} + c - \frac{c^2}{2}) + (\frac{3}{2} + c - \frac{c^2}{2})^2] dx\\
           &= \frac{1}{20}[(1+c)^5 - 1] - \frac{1}{2}[(1+c)^4 - 1] + \frac{4}{3}[(1+c)^3 - 1]\\
           &\ \ \ + \frac{1}{3}[(1+c)^3 - 1](\frac{3}{2} + c - \frac{c^2}{2})
              - 2[(1+c)^2 - 1](\frac{3}{2} + c - \frac{c^2}{2})\\
           &\ \ \ + c(\frac{3}{2} + c - \frac{c^2}{2})^2\\
           &= -\frac{53}{60} + \frac{(1+c)^5}{20} - \frac{(1+c)^4}{2} + \frac{4(1+c)^3}{3}
              + (\frac{c^3}{3} - c^2 -3c)(\frac{3}{2} + c - \frac{c^2}{2})\\
           &\ \ \ + c(\frac{3}{2} + c - \frac{c^2}{2})^2\\
           &= -\frac{53}{60} + \frac{(1+c)^5}{20} - \frac{(1+c)^4}{2} + \frac{4(1+c)^3}{3}
              - (\frac{c^3}{6} + \frac{3c}{2})(\frac{3}{2} + c - \frac{c^2}{2})\\
           &= -\frac{53}{60} + \frac{(1+c)^5}{20} - \frac{(1+c)^4}{2} + \frac{4(1+c)^3}{3}
              + \frac{c^5}{12} - \frac{c^4}{6} + \frac{c^3}{2} - \frac{3c^2}{2} - \frac{9c}{4}
		\end{aligned}
	\end{equation*}
    and
    \begin{equation*}
		\begin{aligned}
		E_3 &= \int_0^1 G_3(c) dc \\
		   &= -\frac{53}{60} + \frac{2^6-1}{120} - \frac{2^5-1}{10} + \frac{2^4-1}{3}
                + \frac{1}{72} - \frac{1}{30} + \frac{1}{8} - \frac{1}{2} - \frac{9}{8} \\
           &= \frac{1}{45}
		\end{aligned}
	\end{equation*}

    Combining $E_1, E_2$, and $E_3$,
    \begin{equation*}
        \mathbb{E}[Z] = E_1 + E_2 + E_3 = \frac{17}{40} + \frac{23}{120} + \frac{1}{45}
                      = \frac{23}{36} = 0.63\overline{8}
    \end{equation*}
\end{document}
